Test/comp/TailRecursion.dfy
@@ -21,6 +21,8 @@ method Main() {
 
   var total := PrintSum(10, 0, "");
   print " == ", total, "\n";
+
+  AutoAccumulatorTests();
 }
 
 method {:tailrecursion} M(n: nat, a: nat) returns (r: nat) {
@@ -74,4 +76,109 @@ method PrintSum(n: nat, acc: nat, prefix: string) returns (total: nat) {
     print prefix, n;
     total := PrintSum(n - 1, n + acc, " + "); // tail recursion
   }
+}
+
+// ----- auto-accumulator tail recursion -----
+
+method AutoAccumulatorTests() {
+  print "TriangleNumber(10) = ", TriangleNumber(10), "\n"; // 55
+  print "TriangleNumber_Real(10) = ", TriangleNumber_Real(10), "\n"; // 55.0
+  print "TriangleNumber_ORDINAL(10) = ", TriangleNumber_ORDINAL(10), "\n"; // 55
+  print "Factorial(5) = ", Factorial(5), "\n";
+  print "Union(8) = ", Union(8), "\n";
+  print "UpTo(10) = ", UpTo(10), "\n";
+  print "DownFrom(10) = ", DownFrom(10), "\n";
+  var xs := Cons(100, Cons(40, Cons(60, Nil)));
+  print "Sum(", xs, ") = ", Sum(xs), "\n";
+  print "TheBigSubtract(100) = ", TheBigSubtract(100), "\n"; // -12
+  print "TailNat(10) = ", TailNat(10), "\n";
+}
+
+function method {:tailrecursion} TriangleNumber(n: nat): nat {
+  if n == 0 then // test if-then-else
+    0
+  else if n % 2 == 0 then
+    TriangleNumber(n - 1) + n // test right accumulator
+  else
+    n + TriangleNumber(n - 1) // test left accumulator
+}
+
+function method {:tailrecursion} TriangleNumber_Real(n: nat): real {
+  if n == 0 then // test if-then-else
+    0.0
+  else
+    TriangleNumber_Real(n - 1) + n as real
+}
+
+function method {:tailrecursion} TriangleNumber_ORDINAL(n: nat): ORDINAL {
+  if n == 0 then // test if-then-else
+    0
+  else
+    TriangleNumber_ORDINAL(n - 1) + n as ORDINAL
+}
+
+function method {:tailrecursion} Factorial(n: nat): nat {
+  if n == 0 then // test if-then-else
+    1
+  else if n % 2 == 0 then
+    Factorial(n - 1) * n // test right accumulator
+  else
+    n * Factorial(n - 1) // test left accumulator
+}
+
+function method {:tailrecursion} Union(n: nat): set<nat> {
+  if n == 0 then // test if-then-else
+    {0}
+  else if n % 2 == 0 then
+    Union(n - 1) + {n} // test right accumulator
+  else
+    {n} + Union(n - 1) // test left accumulator
+}
+
+function method {:tailrecursion} UpTo(n: nat): seq<nat> {
+  if n == 0 then
+    ZeroSeq() // test non-recursive call
+  else
+    UpTo(n - 1) + [n] // test right-accumulator concat
+}
+
+function method {:tailrecursion} DownFrom(n: nat): seq<nat> {
+  if n == 0 then
+    ZeroSeq() // test non-recursive call
+  else
+    [n] + DownFrom(n - 1) // test left-accumulator concat
+}
+
+function method ZeroSeq(): seq<int> {
+  [0]
+}
+
+datatype List = Nil | Cons(head: int, tail: List)
+
+function method {:tailrecursion} Sum(xs: List): int {
+  match xs // test match
+  case Nil =>
+    assert xs.Nil?; // test StmtExpr
+    var zero := 0; // test let expr
+    zero
+  case Cons(x, rest) =>
+    Sum(xs.tail) + xs.head
+}
+
+function method {:tailrecursion} TheBigSubtract(n: nat): int
+  ensures TheBigSubtract(n) == 88 - n
+{
+  if n == 0 then
+    88
+  else
+    TheBigSubtract(n - 1) - 1 // test subtraction accumulation
+}
+
+function method {:tailrecursion} TailNat(n: int): nat
+  requires 0 <= n <= 20
+  ensures TailNat(n) == 100 - 5 * n
+{
+  if n == 0 then 100 else
+    // In this case, the accumulator's value will not be a "nat", but that's okay in the end
+    (-5) + TailNat(n - 1)
 }
